First Hoare logic version with coverage
Nearly all of the pancake language is covered now, and the proofs
aren't too bad.

pancake/semantics/panHoareScript.sml
@@ -48,19 +48,21 @@ QED
 
 Overload local_word = ``\locs nm. OPTION_BIND (FLOOKUP locs nm) val_word_of``
 
+Overload fcopy[local] = ``\nm locs_from locs_to. res_var locs_to (nm, FLOOKUP locs_from nm)``
+
 Definition tick_context_def:
   tick_context context = if NULL context.future_triples then context
     else (context with <| triples := context.future_triples ++ context.triples;
         future_triples := [] |>)
 End
 
-(* should this be presented syntactically via Inductive? *)
 Definition eval_logic_def:
-  eval_logic G P exp v Q = (!s. P s ==> ?x. eval s exp = SOME x /\
-    Q (s with locals := (s.locals |+ (v, x))))
+  eval_logic G P exp v Q = (! s ls. P s ls ==> ?x. eval s exp = SOME x /\
+    Q s (((HD ls) |+ (v, x)) :: DROP 1 ls))
 End
 
 Theorem eval_logic_elim = hd (RES_CANON eval_logic_def)
+Theorem eval_logic_intro = last (RES_CANON eval_logic_def)
 
 Definition opt_op_precond_def:
   opt_op_precond P f Q = (!s. P s ==> ?x. f s = SOME x /\ Q x s)
@@ -99,26 +101,16 @@ Inductive hoare_logic:
 
 [hoare_logic_weaken_pre:]
   (! P Q R.
-    (!s. P s ==> Q s) /\
+    (!s ls. P s ls ==> Q s ls) /\
     hoare_logic G Q p R ==>
     hoare_logic G P p R
   )
 
 [hoare_logic_strengthen_post:]
   (! P Q R.
-    (!res s. Q res s /\ res <> SOME Error ==> R res s) /\
+    (!res s ls. Q res s ls /\ res <> SOME Error ==> R res s ls) /\
     hoare_logic G P p Q ==>
     hoare_logic G P p R
-  )
-
-
-[hoare_logic_equiv:]
-  (! P Q R.
-    (!s r s1. P s /\ evaluate (p, s) = (r, s1) ==>
-        ?s2. evaluate (p2, s) = (r, s2) /\
-        (r <> SOME Error ==> s2.ffi = s1.ffi /\ (R r s2 ==> R r s1))) /\
-    hoare_logic G Q p2 R ==>
-    hoare_logic G (\s. P s /\ Q s) p R
   )
 
 [hoare_logic_Skip:]
@@ -136,19 +128,83 @@ Inductive hoare_logic:
     hoare_logic G (P (SOME Continue)) Continue P
   )
 
+[hoare_logic_Return:]
+  ( !P.
+    eval_logic G P e (strlit "return-val")
+        (\s ls. case FLOOKUP (HD ls) (strlit "return-val") of
+            | NONE => F
+            | SOME v => size_of_shape (shape_of v) <= 32 /\
+                Q (SOME (Return v)) (empty_locals s) (DROP 1 ls)) ==>
+    hoare_logic G (\s ls. P s (FEMPTY :: ls)) (Return e) Q
+  )
+
+[hoare_logic_Raise:]
+  ( !P.
+    eval_logic G P e (strlit "exn-val")
+        (\s ls. case FLOOKUP (HD ls) (strlit "exn-val") of
+            | NONE => F
+            | SOME v => (case FLOOKUP s.eshapes eid of
+                | NONE => F
+                | SOME sh => shape_of v = sh /\ size_of_shape sh <= 32 /\
+                    Q (SOME (Exception eid v)) (empty_locals s) (DROP 1 ls))) ==>
+    hoare_logic G (\s ls. P s (FEMPTY :: ls)) (Raise eid e) Q
+  )
+
+[hoare_logic_Tick:]
+  ( !P.
+    hoare_logic G (\s ls. if s.clock = 0 then P (SOME TimeOut) (empty_locals s) ls
+        else P NONE (dec_clock s) ls) Tick P
+  )
+
+[hoare_logic_Store:]
+  ( !P Q R.
+    eval_logic G P addr_e (strlit "addr") Q /\
+    eval_logic G Q val_e (strlit "val") (\s ls.
+        case local_word (HD ls) (strlit "addr") of
+        | NONE => F
+        | SOME addr =>
+        (case FLOOKUP (HD ls) (strlit "val") of
+        | NONE => F
+        | SOME v =>
+        (case mem_stores addr (flatten v) s.memaddrs s.memory of
+        | NONE => F
+        | SOME m => R NONE (s with memory := m) (DROP 1 ls)))) ==>
+    hoare_logic G (\s ls. P s (FEMPTY :: ls)) (Store addr_e val_e) R
+  )
+
+[hoare_logic_StoreByte:]
+  ( !P Q R.
+    eval_logic G P addr_e (strlit "addr") Q /\
+    eval_logic G Q val_e (strlit "val") (\s ls.
+        case local_word (HD ls) (strlit "addr") of
+        | NONE => F
+        | SOME addr =>
+        (case local_word (HD ls) (strlit "val") of
+        | NONE => F
+        | SOME b =>
+        (case mem_store_byte s.memory s.memaddrs s.be addr (w2w b) of
+        | NONE => F
+        | SOME m => R NONE (s with memory := m) (DROP 1 ls)))) ==>
+    hoare_logic G (\s ls. P s (FEMPTY :: ls)) (StoreByte addr_e val_e) R
+  )
+
 [hoare_logic_Dec:]
   (
     ! P Q R.
-    eval_logic G P e v Q /\
-    hoare_logic G Q p (\res s. res_any v (R res) s)
+    eval_logic G P e v
+        (\s ls. Q (s with locals := fcopy v (HD ls) s.locals)
+            (fcopy v s.locals FEMPTY :: DROP 1 ls)) /\
+    hoare_logic G Q p
+        (\res s ls. R res (s with locals := fcopy v (HD ls) s.locals) (DROP 1 ls))
     ==>
-    hoare_logic G P (Dec v e p) R
+    hoare_logic G (\s ls. P s (FEMPTY :: ls)) (Dec v e p) R
   )
 
 [hoare_logic_Assign:]
   ( ! P Q.
-    eval_logic G P e v (Q NONE) ==>
-    hoare_logic G (\s. P s /\
+    eval_logic G P e v
+        (\s ls. Q NONE (s with locals := fcopy v (HD ls) s.locals) (DROP 1 ls)) ==>
+    hoare_logic G (\s ls. P s (FEMPTY :: ls) /\
             OPTION_MAP shape_of (FLOOKUP s.locals v) =
             SOME (panProps$exp_shape (FMAP_MAP2 (shape_of o SND) s.locals) e))
         (Assign v e) Q
@@ -157,7 +213,7 @@ Inductive hoare_logic:
 [hoare_logic_Seq:]
   (
     ! P Q R.
-    hoare_logic G P p1 (\r s. if r = NONE then Q s else R r s) /\
+    hoare_logic G P p1 (\r s ls. if r = NONE then Q s ls else R r s ls) /\
     hoare_logic G Q p2 R ==>
     hoare_logic G P (Seq p1 p2) R
   )
@@ -165,81 +221,134 @@ Inductive hoare_logic:
 [hoare_logic_If:]
   (
     ! P Q1 Q2 R.
-    eval_logic G P cond_exp cond_nm (\s. local_word s.locals cond_nm <> NONE /\
-        if local_word s.locals cond_nm <> SOME 0w
-        then res_any cond_nm Q1 s else res_any cond_nm Q2 s) /\
+    eval_logic G P cond_exp (strlit "condition") (\s ls.
+        case local_word (HD ls) (strlit "condition") of
+        | NONE => F
+        | SOME w => if w <> 0w then Q1 s (DROP 1 ls) else Q2 s (DROP 1 ls)) /\
     hoare_logic G Q1 p1 R /\
     hoare_logic G Q2 p2 R ==>
-    hoare_logic G (\s. FLOOKUP s.locals cond_nm = NONE /\ P s) (If cond_exp p1 p2) R
+    hoare_logic G (\s ls. P s (FEMPTY :: ls)) (If cond_exp p1 p2) R
   )
 
 [hoare_logic_While:]
   (
-    ! Q.
-    eval_logic G P e cond_nm (\s. local_word s.locals cond_nm <> NONE /\
-        res_any cond_nm (if local_word s.locals cond_nm = SOME 0w
-          then R NONE else if s.clock = 0 then (R (SOME TimeOut) o empty_locals)
-          else (Q o dec_clock)) s) /\
-    hoare_logic G Q p (\r s. case r of NONE => P s | SOME Break => R NONE s
-            | SOME Continue => P s | _ => R r s) ==>
-    hoare_logic G P (While e p) R
+    ! Inv P Q G e p R.
+    (!s ls. Inv s ls ==> P s (FEMPTY :: ls)) /\
+    eval_logic G P e (strlit "condition") (\s ls.
+        case local_word (HD ls) (strlit "condition") of
+        | NONE => F
+        | SOME w => if w = 0w then R NONE s (DROP 1 ls)
+          else if s.clock = 0 then R (SOME TimeOut) (empty_locals s) (DROP 1 ls)
+          else Q (dec_clock s) (DROP 1 ls)) /\
+    hoare_logic G Q p (\r s ls. case r of NONE => Inv s ls | SOME Break => R NONE s ls
+            | SOME Continue => Inv s ls | _ => R r s ls) ==>
+    hoare_logic G Inv (While e p) R
   )
 
 [hoare_logic_TailCall:]
-  ( !vshs prog Q.
+  ( !vshs prog P Q.
     ALL_DISTINCT (MAP FST vshs) /\
-    hoare_logic G Q prog (\res s. case res of
-            | SOME (Return r) => R res (empty_locals s)
-            | SOME (FinalFFI fres) => R res (empty_locals s)
-            | SOME (Exception eid exn) => R res (empty_locals s)
+    eval_logic G P (Struct args) (strlit "args_struct")
+        (\s ls. case FLOOKUP (HD ls) (strlit "args_struct") of
+            | SOME (Struct vs) => LIST_REL (\vsh x. SND vsh = shape_of x) vshs vs /\
+                (if s.clock = 0 then R (SOME TimeOut) (empty_locals s) (DROP 1 ls)
+                    else Q (dec_clock s with locals := (FEMPTY |++ ZIP (MAP FST vshs, vs))) ls)
             | _ => F)
+    /\
+    hoare_logic G Q prog (\res s ls. R res (empty_locals s) (DROP 1 ls) /\
+        (case res of
+            | SOME (Return r) => T
+            | SOME (FinalFFI fres) => T
+            | SOME (Exception eid exn) => T
+            | SOME TimeOut => T
+            | _ => F))
     ==>
-    hoare_logic G (\s. FLOOKUP s.code nm = SOME (vshs, prog) /\
-        (case OPT_MMAP (FLOOKUP s.locals) var_nms of
-            NONE => F
-          | SOME vs => MAP shape_of vs = MAP SND vshs /\
-                (if s.clock = 0 then R (SOME TimeOut) (empty_locals s)
-                    else Q (dec_clock s with locals := (FEMPTY |++ ZIP (MAP FST vshs, vs))))))
-        (Call NONE (Label nm) (MAP Var var_nms)) R
+    hoare_logic G (\s ls. FLOOKUP s.code nm = SOME (vshs, prog) /\ P s (FEMPTY :: ls))
+        (TailCall (Label nm) args) R
   )
 
-(* where do we stash the locals??
-[hoare_logic_RetCall:]
-  ( !ret_shape.
-    hoare_logic G (Call NONE (Label nm) (MAP Var var_nms))
-        (\ret s. case ret of
-            | Return retv => shape_of retv = ret_shape /\ R NONE (
+[hoare_logic_GenCall:]
+  (
+    hoare_logic G P (TailCall (Label nm) args)
+        (\res s ls. case res of
+            | SOME (Return retv) => (case ret of
+                | NONE => R NONE (s with locals := HD ls) (DROP 1 ls)
+                | SOME ret_nm => (case FLOOKUP (HD ls) ret_nm of
+                    | SOME prev_retv => shape_of retv = shape_of prev_retv /\
+                        R NONE (s with locals := (HD ls |+ (ret_nm, retv))) (DROP 1 ls)
+                | NONE => F)
+            )
+            | SOME (FinalFFI _) => R res s (DROP 1 ls)
+            | SOME (Exception _ _) => R res s (DROP 1 ls)
+            | SOME TimeOut => R res s (DROP 1 ls)
+            | _ => F)
     ==>
-    hoare_logic G ..
-        (Call (SOME (SOME ret, NONE)) (Label nm) (MAP Var var_nms)) R
-*)
+    hoare_logic G (\s ls. P s (s.locals :: ls))
+        (Call (SOME (ret, NONE)) (Label nm) args) R
+  )
+
+[hoare_logic_GenCall_Handler:]
+  ( !Q.
+    hoare_logic G P (TailCall (Label nm) args)
+        (\res s ls. case res of
+            | SOME (Return retv) => (case ret of
+                | NONE => R NONE (s with locals := HD ls) (DROP 1 ls)
+                | SOME ret_nm => (case FLOOKUP (HD ls) ret_nm of
+                    | SOME prev_retv => shape_of retv = shape_of prev_retv /\
+                        R NONE (s with locals := (HD ls |+ (ret_nm, retv))) (DROP 1 ls)
+                | NONE => F)
+            )
+            | SOME (FinalFFI _) => R res s (DROP 1 ls)
+            | SOME TimeOut => R res s (DROP 1 ls)
+            | SOME (Exception raised_eid exc_val) => if raised_eid = eid
+                then (FLOOKUP s.eshapes eid = SOME (shape_of exc_val) /\
+                    (case FLOOKUP (HD ls) exc_var of SOME prev => shape_of exc_val = shape_of prev
+                        | _ => F) /\
+                    Q (s with locals := (HD ls |+ (exc_var, exc_val))) (DROP 1 ls))
+                else R res s (DROP 1 ls)
+            | _ => F)
+    /\
+    hoare_logic G Q hprog R
+    ==>
+    hoare_logic G (\s ls. P s (s.locals :: ls))
+        (Call (SOME (ret, (SOME (eid, exc_var, hprog)))) (Label nm) args) R
+  )
+
 
 [hoare_logic_ExtCall:]
-  (
-    hoare_logic G
-    (\s.
-        (case local_word s.locals ptr1_nm of NONE => F | SOME p1 =>
-        (case local_word s.locals len1_nm of NONE => F | SOME l1 =>
-        (case local_word s.locals ptr2_nm of NONE => F | SOME p2 =>
-        (case local_word s.locals len2_nm of NONE => F | SOME l2 =>
-        (case read_bytearray p1 (w2n l1) (mem_load_byte s.memory s.memaddrs s.be)
-            of NONE => F | SOME bs1 =>
-        (case read_bytearray p2 (w2n l2) (mem_load_byte s.memory s.memaddrs s.be)
-            of NONE => F | SOME bs2 =>
-        (let ffi_nm = ExtCall (explode f) in
-        (if explode f = ""
+  ( ! Q.
+    eval_logic G Q (Struct [ptr1_e; len1_e; ptr2_e; len2_e]) (strlit "args_struct")
+        (\s ls. case FLOOKUP (HD ls) (strlit "args_struct") of
+            | SOME (Struct args) =>
+            (case val_word_of (EL 0 args) of NONE => F | SOME p1 =>
+            (case val_word_of (EL 1 args) of NONE => F | SOME l1 =>
+            (case val_word_of (EL 2 args) of NONE => F | SOME p2 =>
+            (case val_word_of (EL 3 args) of NONE => F | SOME l2 =>
+            (case read_bytearray p1 (w2n l1) (mem_load_byte s.memory s.memaddrs s.be)
+                of NONE => F | SOME bs1 =>
+            (case read_bytearray p2 (w2n l2) (mem_load_byte s.memory s.memaddrs s.be)
+                of NONE => F | SOME bs2 =>
+            (let ffi_nm = ExtCall (explode f) in
+            (if explode f = ""
             then R NONE (s with memory := write_bytearray p2 bs2 s.memory s.memaddrs s.be)
+                (DROP 1 ls)
             else (G.ffi_guarantee s.ffi.io_events (ffi_nm, bs1, bs2) /\
             (! rv. G.ffi_rely s.ffi.io_events (ffi_nm, bs1, bs2) rv ==>
                 (case rv of
                     | Oracle_final res =>
-                        R (SOME (FinalFFI (Final_event ffi_nm bs1 bs2 res))) (empty_locals s)
+                        R (SOME (FinalFFI (Final_event ffi_nm bs1 bs2 res)))
+                            (empty_locals s) (DROP 1 ls)
                     | Oracle_return ffi l => LENGTH l = LENGTH bs2 /\
                     let ev = IO_event ffi_nm bs1 (ZIP (bs2, l)) in
                     R NONE (s with <| memory := write_bytearray p2 l s.memory s.memaddrs s.be;
-                        ffi := s.ffi with <| ffi_state := ffi; io_events := s.ffi.io_events ++ [ev] |> |>)))
-        ))))))))))
-    (ExtCall f (Var ptr1_nm) (Var len1_nm) (Var ptr2_nm) (Var len2_nm)) R
+                            ffi := s.ffi with <| ffi_state := ffi; io_events := s.ffi.io_events ++ [ev] |> |>)
+                        (DROP 1 ls))))
+            ))))))))
+            | _ => F
+        )
+    ==>
+    hoare_logic G (\s ls. Q s (FEMPTY :: ls))
+        (ExtCall f ptr1_e len1_e ptr2_e len2_e) R
   )
 
 End
@@ -345,54 +454,78 @@ QED
 
 Theorem hoare_logic_sound:
 
-  ! P p Q.
+  ! G P p Q.
   hoare_logic G P p Q ==>
-  (! s res s'. evaluate (p, s) = (res, s') ==> P s ==>
+  (! s ls res s'. evaluate (p, s) = (res, s') ==> P s ls ==>
     ffi_g_ok G s.ffi ==>
-    res <> SOME Error /\ Q res s' /\ ffi_g_ok G s'.ffi /\ ffi_g_imp G s s'
+    res <> SOME Error /\ Q res s' ls /\ ffi_g_ok G s'.ffi /\ ffi_g_imp G s s'
   )
 
 Proof
 
-  ho_match_mp_tac (Q.SPEC `G` hoare_logic_ind)
+  ho_match_mp_tac hoare_logic_ind
   \\ rpt conj_tac
   \\ rpt (gen_tac ORELSE disch_tac)
 
-  >- (
-    metis_tac []
-  )
-  >- (
-    metis_tac []
-  )
-  >- (
-    fs [] \\ metis_tac []
-  )
-  >- (
-    gs [evaluate_def]
-  )
-  >- (
-    gs [evaluate_def]
-  )
-  >- (
-    gs [evaluate_def]
-  )
+  >~ [`Dec _ _ _`]
   >- (
     fs [evaluate_def]
     \\ drule_then (drule_then assume_tac) eval_logic_elim
     \\ gs []
     \\ rpt (pairarg_tac \\ fs [])
+    \\ fs [FLOOKUP_UPDATE, res_var_def]
     \\ first_x_assum (drule_then drule)
     \\ rw []
-    \\ fs [res_any_def]
+    \\ fs [FLOOKUP_UPDATE, FLOOKUP_pan_res_var_thm]
   )
+
+  >~ [`Assign _ _`]
   >- (
     fs [evaluate_def]
     \\ drule_then (drule_then assume_tac) eval_logic_elim
     \\ gvs []
     \\ imp_res_tac eval_exp_shape
-    \\ fs [is_valid_value_def]
+    \\ fs [is_valid_value_def, FLOOKUP_UPDATE, res_var_def]
     \\ gvs []
   )
+
+  >~ [`panLang$Return _`]
+  >- (
+    fs [evaluate_def]
+    \\ drule_then (drule_then assume_tac) eval_logic_elim
+    \\ gvs [FLOOKUP_UPDATE, empty_locals_def]
+  )
+
+  >~ [`Raise _ _`]
+  >- (
+    fs [evaluate_def]
+    \\ drule_then (drule_then assume_tac) eval_logic_elim
+    \\ gvs [FLOOKUP_UPDATE, empty_locals_def]
+    \\ gvs [CaseEq "option"]
+  )
+
+  >~ [`Tick`]
+  >- (
+    fs [evaluate_def]
+    \\ gvs [CaseEq "bool", empty_locals_def, dec_clock_def]
+  )
+
+
+  >~ [`Store _ _`]
+  >- (
+    fs [evaluate_def]
+    \\ rpt (dxrule_then (drule_then assume_tac) eval_logic_elim \\ fs [])
+    \\ gvs [FLOOKUP_UPDATE, CaseEq "v", CaseEq "word_lab", CaseEq "option"]
+  )
+
+  >~ [`StoreByte _ _`]
+  >- (
+    fs [evaluate_def]
+    \\ rpt (dxrule_then (drule_then assume_tac) eval_logic_elim \\ fs [])
+    \\ gvs [FLOOKUP_UPDATE, CaseEq "v", CaseEq "word_lab", CaseEq "option"]
+  )
+
+  >~ [`Seq _ _`]
   >- (
     fs [evaluate_def]
     \\ pairarg_tac \\ fs []
@@ -401,82 +534,125 @@ Proof
     \\ metis_tac []
   )
 
+  >~ [`If _ _ _`]
   >- (
     fs [evaluate_def]
     \\ drule_then (drule_then assume_tac) eval_logic_elim
     \\ fs [FLOOKUP_UPDATE]
-    \\ imp_res_tac val_word_of_neq_NONE
-    \\ gs []
+    \\ gs [CaseEq "option", CaseEq "v", CaseEq "word_lab"]
     \\ imp_res_tac (Q.prove (`(if P then x else y) ==> (P \/ ~ P)`, metis_tac []))
-    \\ gs []
+    \\ fs []
     \\ first_x_assum (drule_then irule)
-    \\ fs [res_any_drop_update]
-    \\ imp_res_tac res_any_same
+    \\ fs []
   )
+
+  >~ [`While _ _`]
   >- (
     dxrule evaluate_While_inv_final
-    \\ disch_then (qspec_then `\s'. P s' /\ ffi_g_ok G s'.ffi /\ ffi_g_imp G s s'` mp_tac)
+    \\ disch_then (qspec_then `\s'. P' s' (FEMPTY :: ls) /\
+        ffi_g_ok G s'.ffi /\ ffi_g_imp G s s'` mp_tac)
     \\ impl_tac \\ fs []
     >- (
       (* prove invariant preserved *)
       rpt (gen_tac ORELSE disch_tac)
       \\ fs []
-      \\ drule_then (drule_then assume_tac) eval_logic_elim
-      \\ fs [FLOOKUP_UPDATE]
-      \\ imp_res_tac val_word_of_neq_NONE
-      \\ gs [res_any_drop_update]
-      \\ imp_res_tac res_any_same
-      \\ rpt (gen_tac ORELSE disch_tac)
-      \\ fs []
-      \\ first_x_assum (drule_then drule)
-      \\ simp [dec_clock_def]
+      \\ dxrule_then drule eval_logic_elim
+      \\ fs [FLOOKUP_UPDATE, PULL_EXISTS]
+      \\ rpt gen_tac
+      \\ TOP_CASE_TAC
+      \\ fs [val_word_of_eq_SOME]
+      \\ rw [dec_clock_def] \\ res_tac \\ gs []
     )
     \\ simp [PULL_EXISTS]
     \\ gen_tac
-    \\ Cases_on `P fs` \\ fs []
-    \\ dxrule_then (drule_then assume_tac) eval_logic_elim
-    \\ fs [FLOOKUP_UPDATE]
-    \\ imp_res_tac val_word_of_neq_NONE
-    \\ gs [res_any_drop_update]
-    \\ imp_res_tac res_any_same
-    \\ ONCE_REWRITE_TAC [evaluate_def]
-    \\ rw [] \\ gs [empty_locals_def]
-    \\ gs [UNCURRY_eq_pair]
-    \\ last_x_assum (drule_then assume_tac)
-    \\ gs [CaseEq "option", dec_clock_def, CaseEq "result"]
-  )
-
-  >- (
-    (* TailCall *)
-    fs []
-    \\ qpat_x_assum `case _ of NONE => F | _ => _` mp_tac
+    \\ Cases_on `P' fs (FEMPTY :: ls)` \\ fs []
+    \\ dxrule_then drule eval_logic_elim
+    \\ simp [FLOOKUP_UPDATE, PULL_EXISTS]
+    \\ rpt gen_tac
     \\ TOP_CASE_TAC
-    \\ strip_tac
-    \\ gs [evaluate_def, eval_def]
-    \\ fs [OPT_MMAP_MAP_o, o_DEF, eval_def, Q.ISPEC `FLOOKUP _` ETA_THM]
-    \\ fs [lookup_code_def, Q.ISPEC `MAP shape_of _` EQ_SYM_EQ]
-    \\ gs [MAP_EQ_EVERY2]
-    \\ fs [CaseEq "bool"]
-    \\ gvs [] \\ simp [empty_locals_def]
-    \\ fs [CaseEq "prod"]
-    \\ first_x_assum drule
-    \\ simp [dec_clock_def]
-    \\ fs [CaseEq "option", CaseEq "result"] \\ gvs []
-    \\ simp [empty_locals_def]
+    \\ fs [val_word_of_eq_SOME]
+    \\ ONCE_REWRITE_TAC [evaluate_def]
+    \\ fs [empty_locals_def, dec_clock_def]
+    \\ rpt (pairarg_tac \\ fs [])
+    \\ first_x_assum (drule_then (qspec_then `ls` mp_tac))
+    \\ rw [] \\ fs []
+    \\ gs [CaseEq "option", CaseEq "result"] \\ gvs []
   )
 
+  >~ [`evaluate (Call (SOME (ret, NONE)) (Label nm) args, s)`]
   >- (
-    (* ExtCall *)
+    fs []
+    \\ Cases_on `evaluate (TailCall (Label nm) args, s)`
+    \\ first_x_assum (drule_then drule)
+    \\ fs [evaluate_def]
+    \\ gs [CaseEq "option", CaseEq "v", CaseEq "word_lab", CaseEq "prod", CaseEq "bool"]
+    \\ gs [CaseEq "result", CaseEq "option"] \\ gvs []
+    \\ simp [empty_locals_def]
+    \\ TOP_CASE_TAC \\ fs [is_valid_value_def]
+    \\ fs [CaseEq "bool"]
+    \\ gvs [set_var_def]
+  )
+
+  >~ [`evaluate (Call (SOME (ret, SOME (exc_id, exc_var, hprog))) (Label nm) args, s)`]
+  >- (
+    fs []
+    \\ Cases_on `evaluate (TailCall (Label nm) args, s)`
+    \\ first_x_assum (drule_then drule)
+    \\ fs [evaluate_def]
+    \\ gs [CaseEq "option", CaseEq "v", CaseEq "word_lab", CaseEq "prod", CaseEq "bool"]
+    \\ gvs [CaseEq "result", CaseEq "option", empty_locals_def]
+    >- (
+      (* return case *)
+      TOP_CASE_TAC \\ fs [is_valid_value_def]
+      \\ fs [CaseEq "bool"]
+      \\ gvs [set_var_def]
+    )
+    >- (
+      (* exn case *)
+      fs [CaseEq "bool"] \\ gvs []
+      \\ imp_res_tac evaluate_invariants
+      \\ fs [CaseEq "option", dec_clock_def] \\ gs []
+      \\ TOP_CASE_TAC \\ fs [is_valid_value_def]
+      \\ disch_tac \\ gs [CaseEq "bool"]
+      \\ fs [set_var_def]
+      \\ first_x_assum (drule_then drule)
+      \\ simp []
+    )
+  )
+
+  >~ [`TailCall _ _`]
+  >- (
+    fs []
+    \\ dxrule_then drule eval_logic_elim
+    \\ simp [eval_def, Q.ISPEC `eval _` ETA_THM]
+    \\ fs [evaluate_def, eval_def, CaseEq "option", lookup_code_def] \\ gvs []
+    \\ simp [FLOOKUP_UPDATE]
+    \\ fs [CaseEq "bool", CaseEq "prod"] \\ gvs [empty_locals_def]
+    \\ disch_tac
+    \\ first_x_assum (drule_then drule)
+    \\ fs [dec_clock_def]
+    \\ fs [CaseEq "result", CaseEq "option"] \\ gvs []
+  )
+
+  >~ [`ExtCall _ _`]
+  >- (
     fs [evaluate_def, ffiTheory.call_FFI_def, eval_def]
+    \\ dxrule_then drule eval_logic_elim
+    \\ simp [eval_def, FLOOKUP_UPDATE]
+    \\ simp [PULL_EXISTS]
+    \\ TOP_CASE_TAC
+    \\ gvs []
     \\ gs [CaseEq "option", CaseEq "v", CaseEq "word_lab"]
-    \\ Cases_on `explode f = ""`
-    \\ fs []
+    \\ gvs []
+    \\ Cases_on `explode f = ""` \\ fs []
     >- (
       gvs []
-      \\ qsuff_tac `!s t. Q NONE s /\ s = t ==> Q NONE t`
+      \\ disch_tac
+      \\ qsuff_tac `!s t ls. Q NONE s ls /\ s = t ==> Q NONE t ls`
       \\ TRY (disch_then (drule_then irule))
       \\ simp [panSemTheory.state_component_equality]
     )
+    \\ strip_tac
     \\ drule_then drule ffi_rely_guarantee_step
     \\ strip_tac
     \\ first_x_assum drule
@@ -484,6 +660,9 @@ Proof
     \\ rw []
     \\ simp [events_meet_guarantee_snoc, MAP_ZIP, empty_locals_def]
   )
+
+  \\ gs [evaluate_def]
+  \\ metis_tac []
 
 QED
 
@@ -553,35 +732,278 @@ Proof
   \\ simp [FLOOKUP_UPDATE]
 QED
 
-Theorem hoare_logic_ExtCall_add_Decs:
-    ALL_DISTINCT [ptr1_nm; len1_nm; ptr2_nm; len2_nm] /\
-    DISJOINT (set [ptr1_nm; len1_nm; ptr2_nm; len2_nm])
-       (set (FLAT (MAP var_exp (panProps$exps_of p ++ [ptr1_e; len1_e; ptr2_e; len2_e])))) /\
-    DISJOINT (set [ptr1_nm; len1_nm; ptr2_nm; len2_nm])
-       (set (panProps$assigns_of p)) /\
-    hoare_logic G P
-       (Dec ptr1_nm ptr1_e (Dec len1_nm len1_e (Dec ptr2_nm ptr2_e (Dec len2_nm len2_e
-           (ExtCall f (Var ptr1_nm) (Var len1_nm) (Var ptr2_nm) (Var len2_nm)))))) R ==>
-    hoare_logic G (\s. MAP (FLOOKUP s.locals) [ptr1_nm; len1_nm; ptr2_nm; len2_nm] =
-             [NONE; NONE; NONE; NONE] /\ P s)
-        (ExtCall f ptr1_e len1_e ptr2_e len2_e) R
+Definition logic_imp_def:
+  logic_imp P Q = (!s ls. P s ls ==> Q s ls)
+End
+
+Theorem hoare_logic_weaken_imp =
+    REWRITE_RULE [GSYM logic_imp_def] hoare_logic_weaken_pre
+
+Definition annot_While_def:
+  annot_While
+    (Inv : (('a, 'ffi) state -> (mlstring |-> 'a v) list -> bool))
+    (c : 'a panLang$exp) (b : 'a panLang$prog) =
+    panLang$While c b
+End
+
+Theorem hoare_logic_annot_While:
+  logic_imp Inv (\s ls. P s (FEMPTY :: ls)) /\
+  eval_logic G P e (strlit "condition") (\s ls.
+        case local_word (HD ls) (strlit "condition") of
+        | NONE => F
+        | SOME w => if w = 0w then R NONE s (DROP 1 ls)
+          else if s.clock = 0 then R (SOME TimeOut) (empty_locals s) (DROP 1 ls)
+          else Q (dec_clock s) (DROP 1 ls)) /\
+  hoare_logic G Q p (\r s ls. case r of NONE => Inv s ls | SOME Break => R NONE s ls
+        | SOME Continue => Inv s ls | _ => R r s ls) ==>
+  hoare_logic G Inv (annot_While Inv e p) R
 Proof
-  rpt strip_tac
-  \\ ho_match_mp_tac hoare_logic_equiv
-  \\ first_x_assum (irule_at Any)
+  rw [annot_While_def, logic_imp_def]
+  \\ qspec_then `Inv` irule hoare_logic_While
+  \\ rpt (first_assum (irule_at Any))
+  \\ simp []
+QED
+
+
+
+
+Definition exp_args_def:
+  exp_args (Struct xs) = xs /\
+  exp_args (Field ix e) = [e] /\
+  exp_args (Load sh addr) = [addr] /\
+  exp_args (LoadByte addr) = [addr] /\
+  exp_args (Op bop xs) = xs /\
+  exp_args (Panop pop xs) = xs /\
+  exp_args (Cmp cmp x y) = [x; y] /\
+  exp_args (Shift sh_type x n) = [x] /\
+  exp_args _ = []
+End
+
+Definition eval_args_def:
+  eval_args s vs (Const w) = SOME (ValWord w) /\
+  eval_args s vs (Var v) = FLOOKUP s.locals v /\
+  eval_args s vs (Label fname) =
+    OPTION_MAP (\_. ValLabel fname) (FLOOKUP s.code fname) /\
+  eval_args s vs (Struct es) = SOME (Struct vs) /\
+  eval_args s vs (Field index e) = (case LLOOKUP vs 0 of
+    | SOME (Struct vs2) => LLOOKUP vs2 index
+    | _ => NONE) /\
+  eval_args s (vs : ('a v) list) (Load shape addr) = OPTION_BIND (LLOOKUP vs 0)
+    (\v. OPTION_BIND (val_word_of v) (\w. mem_load shape w s.memaddrs s.memory)) /\
+  eval_args s (vs : ('a v) list) (LoadByte addr) = OPTION_BIND (LLOOKUP vs 0)
+    (\v. OPTION_BIND (val_word_of v)
+        (OPTION_MAP (ValWord o w2w) o mem_load_byte s.memory s.memaddrs s.be)) /\
+  eval_args s vs (Op op es) = OPTION_BIND (OPT_MMAP val_word_of vs)
+    (OPTION_MAP ValWord o word_op op) /\
+  eval_args s vs (Panop pop es) = OPTION_BIND (OPT_MMAP val_word_of vs)
+    (OPTION_MAP ValWord o pan_op pop) /\
+  eval_args s vs (Cmp cmp e1 e2) = OPTION_MAP
+    (\ws. ValWord (if OPTREL (word_cmp cmp) (LLOOKUP ws 0) (LLOOKUP ws 1) then 1w else 0w))
+    (OPT_MMAP val_word_of vs) /\
+  eval_args s vs (Shift sh e n) = OPTION_BIND (LLOOKUP vs 0)
+    (\v. OPTION_BIND (val_word_of v) (\w. OPTION_MAP ValWord (word_sh sh w n))) /\
+  eval_args s vs BaseAddr = SOME (ValWord s.base_addr)
+End
+
+Triviality eval_args_thm_helper:
+  OPT_MMAP val_word_of xs = (if EVERY (\x. case x of (ValWord _) => T | _ => F) xs
+    then SOME (MAP (\x. case x of (ValWord w) => w) xs) else NONE)
+Proof
+  Induct_on `xs` \\ simp []
+  \\ Cases \\ simp []
+  \\ Cases_on `w` \\ simp []
+  \\ rpt (TOP_CASE_TAC \\ fs [])
+QED
+
+Theorem eval_args_thm:
+  eval s exp = OPTION_BIND (OPT_MMAP (eval s) (exp_args exp)) (\vs. eval_args s vs exp)
+Proof
+  Cases_on `exp`
+  \\ simp [eval_def, exp_args_def, eval_args_def, Q.ISPEC `eval _` ETA_THM]
+  >~ [`word_op _`]
+  >- (
+    TOP_CASE_TAC \\ simp []
+    \\ simp [eval_args_thm_helper]
+    \\ rw []
+  )
+  >~ [`pan_op _`]
+  >- (
+    TOP_CASE_TAC \\ simp []
+    \\ simp [eval_args_thm_helper]
+    \\ rw []
+  )
+  \\ simp [eval_def, exp_args_def, eval_args_def, Q.ISPEC `eval _` ETA_THM]
+  \\ every_case_tac \\ simp [miscTheory.LLOOKUP_THM]
+QED
+
+Theorem eval_logic_args:
+  eval_logic G P (Struct (exp_args exp)) (strlit "args_struct")
+    (\s ls. case FLOOKUP (HD ls) (strlit "args_struct") of
+        | SOME (Struct vs) => (case eval_args s vs exp of
+            | SOME v => Q s ((HD (DROP 1 ls) |+ (v_nm, v)) :: DROP 2 ls)
+            | NONE => F)
+        | _ => F) ==>
+  eval_logic G (\s ls. P s (FEMPTY :: ls)) exp v_nm Q
+Proof
+  rw []
+  \\ rw [eval_logic_def, eval_args_thm]
+  \\ dxrule_then drule eval_logic_elim
   \\ rw []
-  \\ drule evaluate_ExtCall_add_Decs
-  \\ disch_then (drule_at (Pat `ALL_DISTINCT _`))
-  \\ fs []
-  \\ metis_tac []
+  \\ fs [eval_def, CaseEq "option", FLOOKUP_UPDATE, Q.ISPEC `eval _` ETA_THM]
+  \\ gvs []
+  \\ every_case_tac \\ fs []
 QED
 
 Theorem eval_logic_Const:
-  eval_logic G (\s. Q (s with locals := s.locals |+ (v_nm, ValWord c))) (Const c) v_nm Q
+  eval_logic G (\s ls. Q s ((HD ls |+ (v_nm, ValWord c)) :: DROP 1 ls))
+    (Const c) v_nm Q
 Proof
   simp [eval_logic_def, eval_def]
 QED
 
+Theorem eval_logic_Var:
+  eval_logic G (\s ls. case FLOOKUP s.locals v of
+        NONE => F | SOME x => Q s ((HD ls |+ (v_nm, x)) :: DROP 1 ls))
+    (Var v) v_nm Q
+Proof
+  rw [eval_logic_def, eval_def]
+  \\ every_case_tac \\ fs []
+QED
 
+Theorem eval_logic_Label:
+  eval_logic G (\s ls. case FLOOKUP s.code lab of
+        NONE => F | SOME _ => Q s ((HD ls |+ (v_nm, ValLabel lab)) :: DROP 1 ls))
+    (Label lab) v_nm Q
+Proof
+  rw [eval_logic_def, eval_def]
+  \\ every_case_tac \\ fs []
+QED
+
+Theorem eval_logic_Struct_CONS:
+  eval_logic G P exp (strlit "field") Q /\
+  eval_logic G Q (Struct exps) (strlit "struct")
+    (\s ls. case
+            (FLOOKUP (HD ls) (strlit "field"), FLOOKUP (HD ls) (strlit "struct")) of
+        | (SOME fld, SOME (Struct xs)) => R s ((HD (DROP 1 ls) |+ (v_nm, Struct (fld :: xs))) :: DROP 2 ls)
+        | _ => F)
+  ==>
+  eval_logic G (\s ls. P s (FEMPTY :: ls)) (Struct (exp :: exps)) v_nm R
+Proof
+  rw []
+  \\ irule eval_logic_intro \\ rw []
+  \\ rpt (dxrule_then drule eval_logic_elim \\ rw [])
+  \\ fs [eval_def, FLOOKUP_UPDATE, CaseEq "option"]
+  \\ gvs []
+QED
+
+Theorem eval_logic_Struct_NIL:
+  eval_logic G (\s ls. Q s ((HD ls |+ (v_nm, Struct [])) :: DROP 1 ls)) (Struct []) v_nm Q
+Proof
+  simp [eval_logic_def, eval_def]
+QED
+
+Theorem eval_logic_Field:
+  eval_logic G P str_e (strlit "struct")
+    (\s ls. case FLOOKUP (HD ls) (strlit "struct") of
+        | SOME (Struct xs) => ix < LENGTH xs /\
+            Q s ((HD (DROP 1 ls) |+ (v_nm, EL ix xs)) :: DROP 2 ls)
+        | _ => F)
+  ==>
+  eval_logic G (\s ls. P s (FEMPTY :: ls)) (Field ix str_e) v_nm Q
+Proof
+  rw [] \\ irule eval_logic_intro \\ rw []
+  \\ rpt (dxrule_then drule eval_logic_elim \\ rw [])
+  \\ fs [FLOOKUP_UPDATE, eval_def]
+  \\ every_case_tac \\ fs []
+QED
+
+Theorem eval_logic_Load:
+  eval_logic G P addr_e (strlit "addr")
+    (\s ls. case FLOOKUP (HD ls) (strlit "addr") of
+        | SOME (ValWord x) => (case mem_load shape x s.memaddrs s.memory of
+            | SOME v => Q s ((HD (DROP 1 ls) |+ (v_nm, v)) :: DROP 2 ls)
+            | _ => F)
+        | _ => F)
+  ==>
+  eval_logic G (\s ls. P s (FEMPTY :: ls)) (Load shape addr_e) v_nm Q
+Proof
+  rw [] \\ irule eval_logic_intro \\ rw []
+  \\ rpt (dxrule_then drule eval_logic_elim \\ rw [])
+  \\ fs [FLOOKUP_UPDATE, eval_def]
+  \\ every_case_tac \\ fs []
+QED
+
+Theorem eval_logic_LoadByte:
+  eval_logic G P addr_e (strlit "addr")
+    (\s ls. case FLOOKUP (HD ls) (strlit "addr") of
+        | SOME (ValWord x) => (case mem_load_byte s.memory s.memaddrs s.be x of
+            | SOME v => Q s ((HD (DROP 1 ls) |+ (v_nm, ValWord (w2w v))) :: DROP 2 ls)
+            | _ => F)
+        | _ => F)
+  ==>
+  eval_logic G (\s ls. P s (FEMPTY :: ls)) (LoadByte addr_e) v_nm Q
+Proof
+  rw [] \\ irule eval_logic_intro \\ rw []
+  \\ rpt (dxrule_then drule eval_logic_elim \\ rw [])
+  \\ fs [FLOOKUP_UPDATE, eval_def]
+  \\ every_case_tac \\ fs []
+QED
+
+Theorem eval_logic_Cmp:
+  eval_logic G P x_e (strlit "lhs_expr") P1 /\
+  eval_logic G P1 y_e (strlit "rhs_expr")
+    (\s ls. case (FLOOKUP (HD ls) (strlit "lhs_expr"), FLOOKUP (HD ls) (strlit "rhs_expr")) of
+        | (SOME (ValWord x), SOME (ValWord y)) => Q s ((HD (DROP 1 ls) |+ (v_nm, ValWord (if word_cmp cmp x y then 1w else 0w))) :: DROP 2 ls)
+        | _ => F)
+  ==>
+  eval_logic G (\s ls. P s (FEMPTY :: ls)) (Cmp cmp x_e y_e) v_nm Q
+Proof
+  rw [] \\ irule eval_logic_intro \\ rw []
+  \\ rpt (dxrule_then drule eval_logic_elim \\ rw [])
+  \\ fs [FLOOKUP_UPDATE, eval_def]
+  \\ every_case_tac \\ fs []
+QED
+
+Theorem eval_logic_gen:
+  eval_logic G (\s ls. case eval s expr of NONE => F
+        | SOME v => Q s ((HD ls |+ (v_nm, v)) :: DROP 1 ls))
+    expr v_nm Q
+Proof
+  rw [eval_logic_def]
+  \\ every_case_tac \\ fs []
+QED
+
+Theorem hoare_logic_TailCall_code:
+  ! code.
+    FLOOKUP code nm = SOME (vshs, prog) /\
+    ALL_DISTINCT (MAP FST vshs) /\
+    eval_logic G P (Struct args) (strlit "args_struct")
+        (\s ls. case FLOOKUP (HD ls) (strlit "args_struct") of
+            | SOME (Struct vs) => LIST_REL (\vsh x. SND vsh = shape_of x) vshs vs /\
+                (if s.clock = 0 then R (SOME TimeOut) (empty_locals s) (DROP 1 ls)
+                    else Q (dec_clock s with locals := (FEMPTY |++ ZIP (MAP FST vshs, vs))) ls)
+            | _ => F)
+    /\
+    hoare_logic G Q prog (\res s ls. R res (empty_locals s) (DROP 1 ls) /\
+        (case res of
+            | SOME (Return r) => T
+            | SOME (FinalFFI fres) => T
+            | SOME (Exception eid exn) => T
+            | SOME TimeOut => T
+            | _ => F))
+    ==>
+    hoare_logic G (\s ls. code SUBMAP s.code /\ P s (FEMPTY :: ls))
+        (TailCall (Label nm) args) R
+Proof
+  rw []
+  \\ irule hoare_logic_weaken_pre
+  \\ irule_at Any hoare_logic_TailCall
+  \\ rpt (first_assum (irule_at Any))
+  \\ rw []
+  \\ imp_res_tac FLOOKUP_SUBMAP
+QED
+
+
+val _ = export_theory();
 
 
