pancake/semantics/panPropsScript.sml
@@ -787,11 +787,19 @@ Proof
   \\ metis_tac []
 QED
 
-Theore update_locals_not_vars_eval_eq_alt:
+Theorem update_locals_not_vars_eval_eq_alt:
   (~ MEM n (var_exp e) ==>
-  eval (s with locals := locs |+ (n, w)) e = eval s e)
+  eval (s with locals := locs |+ (n, w)) e = eval (s with locals := locs) e)
   /\
   (s with locals := s.locals) = s
+Proof
+  simp [panSemTheory.state_component_equality]
+  \\ rw []
+  \\ irule EQ_TRANS
+  \\ irule_at Any update_locals_not_vars_eval_eq
+  \\ simp []
+  \\ metis_tac []
+QED
 
 Theorem write_bytearray_update_byte:
   ∀bytes ad ad' m adrs be.
@@ -983,9 +991,9 @@ QED
 
 Theorem update_locals_not_vars_evaluate_eq:
   !prog s res s'.
-  evaluate (prog, s) = (res, s') /\
   ~MEM n (FLAT (MAP var_exp (exps_of prog))) /\
-  ~MEM n (assigns_of prog) ==>
+  ~MEM n (assigns_of prog) /\
+  evaluate (prog, s) = (res, s') ==>
   ?b.
   evaluate (prog, s with locals := s.locals |+ (n, w)) =
   (res, if b then (s' with locals := s'.locals |+ (n, w)) else s') /\
